finish defs of transfer

proof/transfer.v
@@ -1,6 +1,6 @@
 Require Import Metalib.Metatheory.
 
-Require Import algo_new.ott.
+Require Import algo.ott.
 Require Import decl.ott.
 
 
@@ -19,17 +19,23 @@ Notation "s ; x : t" := (cons (pair x t) s)
 Notation "x : A ∈ s" := (binds x A s)
    (at level 65, A at level 52, no associativity) : type_scope.
 
-
 Inductive wf_ss : subst_set -> Prop :=
-| wf_ss_nil : wf_ss nil
-| wf_ss_ex  : forall ex t θ,
-    wf_ss θ -> ex `notin` dom θ 
-    -> ld_mono_type t -> wf_ss (θ ; ex : t).
+  | wf_ss_nil : wf_ss nil
+  | wf_ss_ex : forall x t Θ
+    , wf_ss Θ -> x `notin` dom Θ -> ld_mono_type t
+    -> wf_ss (Θ; x : t)
+.
+
+Lemma wf_uniq : forall Θ,
+    wf_ss Θ -> uniq Θ.
+Proof.
+  induction 1; eauto.
+Qed.
 
 
 Inductive inst_type : subst_set -> la_type -> ld_type -> Prop := 
   | inst_t_tvar : forall θ x, wf_ss θ -> inst_type θ (la_t_tvar_f x) (ld_t_var_f x)
-  | inst_t_evar : forall θ x A, wf_ss θ -> x : A ∈ θ -> inst_type θ (la_t_evar x) A
+  | inst_t_evar : forall θ x t, wf_ss θ -> x : t ∈ θ -> inst_type θ (la_t_evar x) t
   | inst_t_int : forall θ, wf_ss θ -> inst_type θ la_t_int ld_t_int
   | inst_t_arrow : forall θ A' B' A B, 
       inst_type θ A' A -> inst_type θ B' B ->
@@ -40,6 +46,13 @@ Inductive inst_type : subst_set -> la_type -> ld_type -> Prop :=
       inst_type θ (la_t_forall A') (ld_t_forall A)
 .
 
+Lemma inst_t_wf_ss : forall θ t t',
+    inst_type θ t t' -> wf_ss θ.
+Proof.
+  induction 1; pick fresh x'; eauto.
+Qed.
+
+
 Inductive inst_ev : subst_set -> var -> la_typelist -> la_typelist -> ld_worklist -> Prop :=
   | inst_ev_nil : forall θ x, inst_ev θ x la_tl_nil la_tl_nil ld_wl_nil
   | inst_ev_lbs : forall θ x lb lbs wl ubs lb' t', inst_ev θ x lbs ubs wl -> 
@@ -48,12 +61,28 @@ Inductive inst_ev : subst_set -> var -> la_typelist -> la_typelist -> ld_worklis
       inst_type θ ub ub' -> inst_type θ (la_t_evar x) t' -> inst_ev θ x lbs (la_tl_cons ubs ub) (ld_wl_cons_w wl (ld_w_sub t' ub'))
 .
 
+Inductive inst_worl : Prop.
+
 
 Inductive inst_worklist : subst_set -> la_worklist -> ld_worklist -> subst_set -> Prop := 
-  | inst_wl_nil  : forall Θ, wf_ss Θ -> inst_worklist Θ la_wl_nil ld_wl_nil Θ
-  | inst_wl_sub : forall θ θ' awl dwl t1 t2 t1' t2', inst_worklist θ awl dwl θ' -> inst_type θ' t1 t1' -> inst_type θ' t2 t2' -> 
-       inst_worklist θ (la_wl_cons_w awl (la_w_sub t1 t2)) (ld_wl_cons_w dwl (ld_w_sub t1' t2')) θ'
-  | inst_wl_tv : forall θ θ' x awl dwl, inst_worklist θ awl dwl θ' -> inst_worklist θ (la_wl_cons_tv awl x) (ld_wl_cons_tv dwl x) θ'
-  | inst_wl_ev : forall θ θ' t lbs ex ubs awl dwl' dwl, inst_worklist θ awl dwl θ' -> ld_wf_mtype (ld_wl_to_ctx dwl) t -> inst_ev (θ' ; ex : t) ex lbs ubs dwl' -> 
-      inst_worklist θ (la_wl_cons_w awl (la_w_evar lbs ex ubs)) (ld_wl_app dwl dwl')  (θ' ; ex : t)
+  | inst_wl_nil : forall θ, 
+      wf_ss θ -> inst_worklist θ la_wl_nil ld_wl_nil θ
+  | inst_wl_sub : forall θ θ' awl dwl t1 t2 t1' t2', 
+      inst_worklist θ awl dwl θ' -> 
+      inst_type θ' t1 t1' -> 
+      inst_type θ' t2 t2' -> 
+      inst_worklist θ (la_wl_cons_w awl (la_w_sub t1 t2)) (ld_wl_cons_w dwl (ld_w_sub t1' t2')) θ'
+  | inst_wl_tv : forall θ θ' x awl dwl, 
+      inst_worklist θ awl dwl θ' -> 
+      inst_worklist θ (la_wl_cons_tv awl x) (ld_wl_cons_tv dwl x) θ'
+  | inst_wl_ev : forall θ θ' t lbs ex ubs awl dwl' dwl, 
+      inst_worklist θ awl dwl θ' -> 
+      ld_wf_mtype (ld_wl_to_ctx dwl) t -> 
+      ex `notin` dom θ' -> 
+      inst_ev (θ' ; ex : t) ex lbs ubs dwl' -> 
+      inst_worklist θ (la_wl_cons_ev awl lbs ex ubs) (ld_wl_app dwl dwl')  (θ' ; ex : t)
 .
+
+
+Definition transfer' (Γ : la_worklist) (Γ' : ld_worklist) : Prop :=
+  exists θ', inst_worklist nil Γ Γ' θ'.
