proof/completeness.v
@@ -1,0 +1,8 @@
+Require Import algo.ott.
+Require Import decl.ott.
+Require Import transfer.
+
+
+Theorem completeness : forall Γ', ld_worklist_reducible Γ' -> exists Γ, transfer' Γ Γ' /\ la_worklist_reducible Γ.
+Proof.
+Admitted.
