proof/soundness.v
@@ -1,1 +1,15 @@
-Require Import decl.notations.
+Require Import Program.Equality.
+
+Require Import algo.ott.
+Require Import decl.ott.
+Require Import transfer.
+
+
+Theorem soundness : forall Γ, la_worklist_reducible Γ -> exists Γ', transfer' Γ Γ' /\ ld_worklist_reducible Γ'.
+Proof.
+  intros. induction H.
+  - destruct IHla_worklist_reducible as [dwl Hdwl]. destruct Hdwl.
+    exists (ld_wl_cons_tv dwl x5). split. 
+    + dependent destruction H1. econstructor. econstructor. eauto.
+    + econstructor; eauto. simpl. econstructor. admit. admit.
+Admitted.
